CoqOfRust/examples/default/examples/rust_book/traits/hash.v
@@ -27,7 +27,6 @@ Section Impl_core_hash_Hash_for_hash_Person_t.
   *)
   Definition hash
       {__H : Set}
-      {ℋ_0 : core.hash.Hasher.Trait __H}
       (self : ref Self)
       (state : mut_ref __H)
       : M unit :=
@@ -64,16 +63,13 @@ Section Impl_core_hash_Hash_for_hash_Person_t.
     let* α0 : M.Val unit := M.alloc α3 in
     M.read α0.
   
-  Global Instance AssociatedFunction_hash
-      {__H : Set}
-      {ℋ_0 : core.hash.Hasher.Trait __H} :
+  Global Instance AssociatedFunction_hash {__H : Set} :
     Notations.DoubleColon Self "hash" := {
     Notations.double_colon := hash (__H := __H);
   }.
   
   Global Instance ℐ : core.hash.Hash.Required.Trait Self := {
-    core.hash.Hash.hash {__H : Set} {ℋ_0 : core.hash.Hasher.Trait __H} :=
-      hash (__H := __H);
+    core.hash.Hash.hash {__H : Set} := hash (__H := __H);
     core.hash.Hash.hash_slice := Datatypes.None;
   }.
 End Impl_core_hash_Hash_for_hash_Person_t.
@@ -86,11 +82,7 @@ fn calculate_hash<T: Hash>(t: &T) -> u64 {
     s.finish()
 }
 *)
-Definition calculate_hash
-    {T : Set}
-    {ℋ_0 : core.hash.Hash.Trait T}
-    (t : ref T)
-    : M u64.t :=
+Definition calculate_hash {T : Set} (t : ref T) : M u64.t :=
   let* t := M.alloc t in
   let* s : M.Val std.hash.random.DefaultHasher.t :=
     let* α0 : std.hash.random.DefaultHasher.t :=
