CoqOfRust/examples/axiomatized/examples/rust_book/functions/functions_closures_type_anonymity_define.v
@@ -23,6 +23,4 @@ Parameter main : M unit.
         f();
     }
 *)
-Parameter apply :
-    forall {F : Set} {ℋ_0 : core.ops.function.FnOnce.Trait F (Args := unit)},
-    F -> M unit.
+Parameter apply : forall {F : Set}, F -> M unit.
