CoqOfRust/examples/axiomatized/examples/rust_book/std_misc/file_io_read_lines_efficient_method.v
@@ -11,7 +11,7 @@ where
 }
 *)
 Parameter read_lines :
-    forall {P : Set} {ℋ_0 : core.convert.AsRef.Trait P (T := std.path.Path.t)},
+    forall {P : Set},
     P ->
       M
         ltac:(std.io.error.Result
