CoqOfRust/examples/axiomatized/examples/rust_book/traits/hash.v
@@ -25,20 +25,15 @@ Section Impl_core_hash_Hash_for_hash_Person_t.
   (*
   Hash
   *)
-  Parameter hash :
-      forall {__H : Set} {ℋ_0 : core.hash.Hasher.Trait __H},
-      (ref Self) -> (mut_ref __H) -> M unit.
+  Parameter hash : forall {__H : Set}, (ref Self) -> (mut_ref __H) -> M unit.
   
-  Global Instance AssociatedFunction_hash
-      {__H : Set}
-      {ℋ_0 : core.hash.Hasher.Trait __H} :
+  Global Instance AssociatedFunction_hash {__H : Set} :
     Notations.DoubleColon Self "hash" := {
     Notations.double_colon := hash (__H := __H);
   }.
   
   Global Instance ℐ : core.hash.Hash.Required.Trait Self := {
-    core.hash.Hash.hash {__H : Set} {ℋ_0 : core.hash.Hasher.Trait __H} :=
-      hash (__H := __H);
+    core.hash.Hash.hash {__H : Set} := hash (__H := __H);
     core.hash.Hash.hash_slice := Datatypes.None;
   }.
 End Impl_core_hash_Hash_for_hash_Person_t.
@@ -51,9 +46,7 @@ fn calculate_hash<T: Hash>(t: &T) -> u64 {
     s.finish()
 }
 *)
-Parameter calculate_hash :
-    forall {T : Set} {ℋ_0 : core.hash.Hash.Trait T},
-    (ref T) -> M u64.t.
+Parameter calculate_hash : forall {T : Set}, (ref T) -> M u64.t.
 
 (*
 fn main() {
