CoqOfRust/examples/default/examples/rust_book/scoping_rules/scoping_rules_lifetimes_bounds.v
@@ -60,7 +60,7 @@ where
     println!("`print`: t is {:?}", t);
 }
 *)
-Definition print {T : Set} {ℋ_0 : core.fmt.Debug.Trait T} (t : T) : M unit :=
+Definition print {T : Set} (t : T) : M unit :=
   let* t := M.alloc t in
   let* _ : M.Val unit :=
     let* _ : M.Val unit :=
@@ -90,11 +90,7 @@ where
     println!("`print_ref`: t is {:?}", t);
 }
 *)
-Definition print_ref
-    {T : Set}
-    {ℋ_0 : core.fmt.Debug.Trait T}
-    (t : ref T)
-    : M unit :=
+Definition print_ref {T : Set} (t : ref T) : M unit :=
   let* t := M.alloc t in
   let* _ : M.Val unit :=
     let* _ : M.Val unit :=
