CoqOfRust/examples/default/examples/rust_book/std_misc/file_io_read_lines_efficient_method.v
@@ -12,7 +12,6 @@ where
 *)
 Definition read_lines
     {P : Set}
-    {ℋ_0 : core.convert.AsRef.Trait P (T := std.path.Path.t)}
     (filename : P)
     :
       M
